theories/Interp/Fold.v
@@ -19,6 +19,12 @@ Open Scope ctree_scope.
 
 (* end hide *)
 
+(* TO MOVE *)
+Ltac cstep :=
+  match goal with
+  |- context[elem ?R] => apply (b_chain R)
+  end.
+
 (** ** Fold *)
 
 (** The most general shape of fold over the structure takes two parameters:
@@ -28,17 +34,23 @@ Open Scope ctree_scope.
     for any monad [M] with a loop operator. *)
 Definition fold {E B M : Type -> Type}
            {FM : Functor M} {MM : Monad M} {IM : MonadIter M}
-           (h : E ~> M) (g : bool -> (B01 +' B) ~> M) :
-  ctree E (B01 +' B) ~> M :=
+           (mstuck : forall X, M X)
+           (mstep : M unit)
+           (h : E ~> M)
+           (g : B ~> M) :
+  ctree E B ~> M :=
   fun R =>
     iter (fun t =>
-	    match observe t with
-	    | RetF r => ret (inr r)
-	    | BrF b c k => fmap (fun x => inl (k x)) (g b _ c)
-	    | VisF e k => fmap (fun x => inl (k x)) (h _ e)
-	    end).
+	          match observe t with
+	          | RetF r => ret (inr r)
+            | StuckF => mstuck _
+            | GuardF t => ret (inl t)
+            | StepF t => fmap (fun _ => inl t) mstep
+	          | BrF c k => fmap (fun x => inl (k x)) (g _ c)
+	          | VisF e k => fmap (fun x => inl (k x)) (h _ e)
+	          end).
 
-Arguments fold {E B M FM MM IM} h g [T].
+Arguments fold {E B M FM MM IM} mstuck mstep h g [T].
 
 (** Implementing simultaneously external events while refining
     the internal non-determinism is somewhat uncommon.
@@ -50,16 +62,25 @@ Arguments fold {E B M FM MM IM} h g [T].
  *)
 
 Definition interp {E B M : Type -> Type}
-           {FM : Functor M} {MM : Monad M} {IM : MonadIter M} {BM : MonadBr B M}
-           (h : E ~> M) := fold h (fun b _ c => mbr b c).
+  {FM : Functor M} {MM : Monad M}
+  {IM : MonadIter M}
+  {Mstuck : MonadStuck M}
+  {Mstep : MonadStep M}
+  {Mbranch : MonadBr B M}
+  (h : E ~> M) : ctree E B ~> M :=
+  fold mstuck mstep h mbr.
 
-Arguments interp {E B M FM MM IM BM} h [T].
+Arguments interp {E B M FM MM IM _ _ _} h [T].
 
 Definition refine {E B M : Type -> Type}
-           {FM : Functor M} {MM : Monad M} {IM : MonadIter M} {TM : MonadTrigger E M}
-           (g : bool -> B01 +' B ~> M) := fold (fun _ e => mtrigger e) g.
+  {FM : Functor M} {MM : Monad M} {IM : MonadIter M} {TM : MonadTrigger E M}
+  {Mstuck : MonadStuck M}
+  {Mstep : MonadStep M}
+  (g : B ~> M)
+  :=
+  fold mstuck mstep (fun _ e => mtrigger e) g.
 
-Arguments refine {E B M FM MM IM TM} g [T].
+Arguments refine {E B M FM MM IM TM _ _} g [T].
 
 Definition translateF {E F C R}
            (h : E ~> F)
@@ -67,8 +88,11 @@ Definition translateF {E F C R}
            (t : ctreeF E C R _) : ctree F C R  :=
   match t with
   | RetF x => Ret x
+  | StuckF => Stuck
+  | StepF t => Step (rec t)
+  | GuardF t => Guard (rec t)
   | VisF e k => Vis (h _ e) (fun x => rec (k x))
-  | BrF b c k => Br b c (fun x => rec (k x))
+  | BrF c k => Br c (fun x => rec (k x))
   end.
 
 Definition translate {E F C} (h : E ~> F) : ctree E C ~> ctree F C
@@ -78,13 +102,22 @@ Arguments translate {E F C} h [T].
 
 (** Useful congruences and lemmas for [interp] and [refine] *)
 #[global] Instance interp_equ {E F B C X} `{HasB: B -< C} h:
-  Proper (equ eq ==> @equ F (B01 +' C) X X eq) (@interp E B _ _ _ _ _ h X).
+  Proper (equ eq ==> @equ F C X X eq)
+    (@interp E B _ _ _ _ _ _ _ h X).
 Proof.
   cbn.
   coinduction R CH.
   intros. setoid_rewrite unfold_iter.
   step in H. inv H; setoid_rewrite <- H1; setoid_rewrite <- H2.
-  - setoid_rewrite bind_ret_l. reflexivity.
+  - now setoid_rewrite bind_ret_l.
+  - now setoid_rewrite bind_stuck.
+  - setoid_rewrite bind_ret_l.
+    constructor; eauto.
+  - setoid_rewrite bind_map.
+    setoid_rewrite bind_step.
+    constructor; rewrite ! bind_ret_l.
+    cstep; constructor.
+    eauto.
   - setoid_rewrite bind_bind. setoid_rewrite bind_ret_l.
     upto_bind_eq.
     constructor. intros.
@@ -92,40 +125,52 @@ Proof.
   - setoid_rewrite bind_bind.
     upto_bind_eq.
     setoid_rewrite bind_ret_l.
-    constructor. intros _.
+    constructor.
     apply CH. apply REL.
 Qed.
 
 #[global] Instance refine_equ {E C X} h:
-  Proper (equ eq ==> @equ E (B01 +' C) X X eq) (@refine E C _ _ _ _ _ h X).
+  Proper (equ eq ==> @equ E C X X eq) (@refine E C _ _ _ _ _ _ _ h X).
 Proof.
   cbn.
   coinduction R CH.
   intros. setoid_rewrite unfold_iter.
   step in H. inv H; setoid_rewrite <- H1; setoid_rewrite <- H2.
-  - setoid_rewrite bind_ret_l. reflexivity.
+  - now setoid_rewrite bind_ret_l.
+  - now setoid_rewrite bind_stuck.
+  - setoid_rewrite bind_ret_l.
+    constructor; eauto.
+  - setoid_rewrite bind_map.
+    setoid_rewrite bind_step.
+    constructor; rewrite ! bind_ret_l.
+    cstep; constructor.
+    eauto.
   - setoid_rewrite bind_bind. setoid_rewrite bind_trigger.
     constructor. intros.
     setoid_rewrite bind_ret_l.
-    step. constructor. intros _.
+    cstep. constructor.
     apply CH. apply REL.
   - setoid_rewrite bind_bind.
     upto_bind_eq.
     setoid_rewrite bind_ret_l.
-    constructor. intros _.
+    constructor.
     apply CH. apply REL.
 Qed.
 
 (** [translate] lemmas *)
 
 (** Unfolding of [translate]. *)
-Notation translate_ h t := (match observe t with
-                            | RetF x => Ret x
-                            | VisF e k => Vis (h _ e) (fun x => translate h (k x))
-                            | BrF b c k => Br b c (fun x => translate h (k x))
-                            end).
+Notation translate_ h t :=
+  (match observe t with
+   | RetF x => Ret x
+   | StuckF => Stuck
+   | StepF t => Step (translate h t)
+   | GuardF t => Guard (translate h t)
+   | VisF e k => Vis (h _ e) (fun x => translate h (k x))
+   | BrF c k => Br c (fun x => translate h (k x))
+   end).
 (** Unfold lemma. *)
-Lemma unfold_translate {E F C X}(t: ctree E C X)(h: E ~> F):
+Lemma unfold_translate {E F C X} (t: ctree E C X) (h: E ~> F):
   translate h t ≅ translate_ h t.
 Proof.
   intros; step; cbn; auto.
@@ -135,20 +180,31 @@ Lemma translate_ret {E F C X}(x: X)(h: E ~> F):
   @translate E F C h X (Ret x) ≅ Ret x.
 Proof. now rewrite unfold_translate. Qed.
 
+Lemma translate_stuck {E F C X}(x: X)(h: E ~> F):
+  @translate E F C h X Stuck ≅ Stuck.
+Proof. now rewrite unfold_translate. Qed.
+
+Lemma translate_guard {E F C X} (t: ctree E C X) (h: E ~> F):
+  @translate E F C h X (Guard t) ≅ Guard (translate h t).
+Proof. now rewrite unfold_translate. Qed.
+
+Lemma translate_step {E F C X} (t: ctree E C X) (h: E ~> F):
+  @translate E F C h X (Step t) ≅ Step (translate h t).
+Proof. now rewrite unfold_translate. Qed.
+
 Lemma translate_vis {E F C X U} (e: E U)(k: U -> ctree E C X)(h: E ~> F):
   @translate E F C h X (Vis e k) ≅ Vis (h _ e) (fun x => translate h (k x)).
 Proof. now rewrite unfold_translate. Qed.
 
-
-Lemma translate_br {E F C X U} b (c : C U) (k: _ -> ctree E C X)(h: E ~> F):
-  @translate E F C h X (Br b c k) ≅ Br b c (fun x => translate h (k x)).
+Lemma translate_br {E F C X U} (c : C U) (k: _ -> ctree E C X)(h: E ~> F):
+  @translate E F C h X (Br c k) ≅ Br c (fun x => translate h (k x)).
 Proof. now rewrite unfold_translate. Qed.
 
 #[global] Instance translate_equ {E F C X} (h: E ~> F):
   Proper (equ eq ==> equ eq) (@translate E F C h X).
 Proof.
   cbn.
-  coinduction ? CIH.
+  coinduction r CIH.
   intros * EQ; step in EQ.
   rewrite 2 unfold_translate.
   inv EQ; auto; constructor; intros; auto.
