theories/Core/CTreeDefinitions.v
@@ -379,6 +379,7 @@ Infinite taus.
 End CTree.
 
 Notation trigger e := (CTree.trigger (subevent _ e)).
+Notation branch  e := (CTree.branch (subevent _ e)).
 
 (*|
 =========
@@ -420,17 +421,17 @@ Instances
 #[global] Instance MonadIter_ctree {E B} : MonadIter (ctree E B) :=
   fun R I => @CTree.iter E B R I.
 
-(* #[global] Instance MonadTrigger_ctree {E B} : MonadTrigger E (ctree E B) | 1 := *)
-(*   @CTree.trigger _ _. *)
-
 #[global] Instance MonadTrigger_ctree {E F B} `{E -< F} : MonadTrigger E (ctree F B) :=
   fun _ e => trigger e.
 
-(* #[global] Instance MonadBr_ctree {E B} : MonadBr B (ctree E B) | 1 := *)
-(*   @CTree.branch _ _. *)
+#[global] Instance MonadBr_ctree {E C D} `{C -< D} : MonadBr C (ctree E D) :=
+  fun _ c => branch c.
 
-(* #[global] Instance MonadBr_ctree {E C D} `{C -< D} : MonadBr C (ctree E D). *)
-(*   fun b _ c => @CTree.branch E B  c. *)
+#[global] Instance MonadStuck_ctree {E C} : MonadStuck (ctree E C) :=
+  fun _ => Stuck.
+
+#[global] Instance MonadStep_ctree {E C} : MonadStep (ctree E C) :=
+  Step (Ret tt).
 
 (*|
 ====================================
