theories/Eq.v
@@ -76,14 +76,14 @@ The three variants are:
 are identical: assumes [reflexivity] will solve the first goal, and proceed to substitute the equality
 - [upto_bind with SS]: for [equ], provides explicitly the intermediate relation
 |*)
-(* #[global] Tactic Notation "upto_bind" := *)
-(*   __eupto_bind_equ || __upto_bind_sbisim || __upto_bind_ssim eq || __upto_bind_cssim. *)
+#[global] Tactic Notation "upto_bind" :=
+  __eupto_bind_equ || __eupto_bind_sbisim.
 
-(* #[global] Tactic Notation "upto_bind_eq" := *)
-(*   __upto_bind_eq_equ || __upto_bind_eq_sbisim || __upto_bind_eq_ssim eq || __upto_bind_eq_cssim. *)
+#[global] Tactic Notation "upto_bind_eq" :=
+  __upto_bind_equ_eq || __upto_bind_sbisim_eq.
 
-(* #[global] Tactic Notation "upto_bind" "with" uconstr(SS) := *)
-(*   __upto_bind_equ SS. *)
+#[global] Tactic Notation "upto_bind" "with" uconstr(SS) :=
+  __upto_bind_equ SS || __upto_bind_sbisim SS.
 
 (*|
 Weakens equalities into respectively [equ] and [sbisim] equations ---
